yet another refactor

src/Node.v
@@ -3,6 +3,7 @@ From Coq Require Import Strings.String.
 
 Definition eqb_string (x y : string) : bool :=
   if string_dec x y then true else false.
+
  (* literals should be of Datatype type, is not important for the moment*)
 Inductive node : Type :=
   | Iri (id: string)
@@ -12,19 +13,19 @@ Inductive node : Type :=
 Definition is_lit (n : node) : bool :=
   (match n with
    | Lit _ => true
-   | otherwise => false
+   | _ => false
    end).
 
 Definition is_iri (n : node) : bool :=
   (match n with
    | Iri _ => true
-   | otherwise => false
+   | _ => false
    end).
 
 Definition is_bnode (n : node) : bool :=
   (match n with
    | Bnode _ => true
-   | otherwise => false
+   | _ => false
    end).
 
 Definition eqb_node (n1 n2 : node) : bool :=
@@ -32,5 +33,5 @@ Definition eqb_node (n1 n2 : node) : bool :=
    | (Iri id), (Iri id2) => eqb id id2
    | (Lit l),(Lit l2) => l =? l2
    | (Bnode b),(Bnode b2) => eqb b b2
-   | e1,e2 => false
+   | _,_ => false
    end).
