src/examples/RdfExamples.v
@@ -5,24 +5,24 @@ From Coq Require Import Lists.ListSet.
 
 Check (triple (Bnode "a") (Lit 1) (Iri "foo")): trpl.
 
-Check (set_add eq_or_not (Iri "x") (set_add eq_or_not (Lit 5) (empty_set node))).
+Check (set_add eq_dec_node (Iri "x") (set_add eq_dec_node (Lit 5) (empty_set node))).
 
-Example example_in_graph : set_In (Lit 12) (set_add eq_or_not (Lit 12) (set_add eq_or_not (Lit 5) (empty_set node))).
-Proof. simpl. destruct (eq_or_not (Lit 12) (Lit 5)) eqn:E.
+Example example_in_graph : set_In (Lit 12) (set_add eq_dec_node (Lit 12) (set_add eq_dec_node (Lit 5) (empty_set node))).
+Proof. simpl. destruct (eq_dec_node (Lit 12) (Lit 5)) eqn:E.
   - simpl. left. symmetry. apply e.
   - simpl. right. left. reflexivity.
 Qed.
 
-Check (set_add eq_or_not_triple (triple (Lit 1) (Lit 1) (Lit 1)) (empty_set trpl)): graph.
+Check (set_add eq_dec_triple (triple (Lit 1) (Lit 1) (Lit 1)) (empty_set trpl)): graph.
 
 (* image of mapping Const 2 of 1,1,1 => 2,1,2*)
-Compute (image (set_add eq_or_not_triple (triple (Lit 1) (Lit 1) (Lit 1)) (empty_set trpl)) 
+Compute (image (set_add eq_dec_triple (triple (Lit 1) (Lit 1) (Lit 1)) (empty_set trpl)) 
   (fun _ => Lit 2)): graph.
 
 Example eqb_graph_test : 
   eqb_graph (empty_set trpl) (empty_set trpl) = true.
 Proof. reflexivity. Qed.
 Example eqb_graph_test2 : 
-  eqb_graph (set_add eq_or_not_triple (triple (Lit 5) (Lit 4) (Lit 3)) (empty_set trpl)) (empty_set trpl) = false.
+  eqb_graph (set_add eq_dec_triple (triple (Lit 5) (Lit 4) (Lit 3)) (empty_set trpl)) (empty_set trpl) = false.
 Proof. reflexivity. Qed.
 
